Admitted bind theorem for pick

src/coq/Handlers/Pick.v
@@ -2383,7 +2383,74 @@ Module Make (LP : LLVMParams) (MP : MemoryParams LP) (Byte : ByteModule LP.ADDR 
       Definition exec_undef `{FailureE -< E +' F} `{UBE -< E +' F} `{OOME -< E +' F} :
         itree (E +' PickE +' F) ~> itree (E +' F) :=
         interp pick_exec_h.
+        Check exec_undef.
+        Print ">>=".
+        Print VisF.
+        Definition _exec_undef {R X Y Post} `{FailureE -< E +' F} `{UBE -< E +' F} `{OOME -< E +' F} 
+          (f : (E +' (@PickE X Y Post) +' F) ~> itree (E +' F)) (ot : itreeF (E +' (@PickE X Y Post) +' F) R _)
+        : itree (E +' F) R :=
+        match ot with
+        | RetF r => Ret r
+        | TauF t => Tau (exec_undef t)
+        | VisF _ e k => f _ e >>= (fun x => Tau (exec_undef (k x)))
+        end.
 
+        Lemma unfold_exec_undef {R} `{FailureE -< E +' F} `{UBE -< E +' F} `{OOME -< E +' F} 
+  h (t: itree (E +' PickE +' F) R):
+ eq_itree eq
+   (exec_undef t)
+    (_exec_undef h (observe t)).
+Proof.
+Import ITree.Eq.Paco2.
+      Import gpacotac.
+
+unfold exec_undef, pick_exec_h, concretize_picks.
+cbn.
+
+rewrite InterpFacts.unfold_interp.
+destruct (observe t); cbn.
+- reflexivity.
+- admit.
+- admit.
+Admitted.
+
+        Lemma exec_undef_bind {T U} `{FailureE -< E +' F} `{UBE -< E +' F} `{OOME -< E +' F}: forall a b,
+        exec_undef (ITree.bind a b) ≅ 
+          ITree.bind (T:= T) (U := U) (exec_undef a) (fun x => exec_undef (b x)).
+      Proof.
+      (* intros. *)
+      Import ITree.Eq.Paco2.
+      Import gpacotac.
+
+      ginit.
+      pcofix CIH.
+      intros.
+      rewrite unfold_exec_undef.
+      rewrite unfold_exec_undef.
+      setoid_rewrite unfold_exec_undef.
+      all: rewrite Shallow.observe_bind.
+      
+      destruct (observe a) eqn: Ha; cbn.
+      rewrite bind_ret_l.
+      cbn.
+      destruct (observe (b _)) eqn: Hb1; cbn.
+      - gstep. reflexivity.
+      - gstep. reflexivity.
+      - gstep. unfold exec_undef. unfold pick_exec_h. admit.
+      - gstep. admit.
+      - setoid_rewrite bind_bind. admit.
+      Unshelve.
+      Admitted.
+
+    Lemma exec_undef_ret {R2} `{FailureE -< E +' F} `{UBE -< E +' F} `{OOME -< E +' F}: forall r, 
+      eq_itree (R2 := R2) eq (exec_undef (Ret r)) (Ret r).
+      Proof.
+      intros.
+      tau_steps.
+      reflexivity.
+      Qed.
+    
+      
     End PARAMS_INTERP.
 
   End PickImplementation.
